Logical relation for normalization STLC

theories/opsem_stlc.v
@@ -1,40 +1,21 @@
 Set Warnings "-notation-overridden,-parsing,-deprecated-hint-without-locality".
 From Coq Require Import Strings.String.
 From stdpp Require Import gmap list.
-From logical_relation Require Import relation syntax_systemF.
+From logical_relation Require Import relation syntax_stlc.
 
 Reserved Notation "t '~>' t'" (at level 60).
 Inductive step : expr -> expr -> Prop :=
-| step_fst_red : forall v1 v2,
-  is_val v1 ->
-  is_val v2 ->
-  <{ fst ⟨ v1, v2 ⟩ }> ~>  <{ v1 }>
-| step_snd_red : forall v1 v2,
-  is_val v1 ->
-  is_val v2 ->
-  <{ snd ⟨ v1, v2 ⟩ }> ~>  <{ v2 }>
+| step_if_true : forall e1 e2,
+  <{ if true then e1 else e2 }> ~>  <{ e1 }>
+| step_if_false : forall e1 e2,
+  <{ if false then e1 else e2 }> ~>  <{ e2 }>
 | step_lam_red : forall x e v,
   is_val v ->
   <{ (λ x, e) v }> ~>  <{ [x / v]e }>
-| step_tlam_red : forall e,
-  <{ (Λ e) _ }> ~>  <{ e }>
-| step_fst : forall e e',
+
+| step_if : forall e e' e1 e2,
   e ~> e' ->
-  <{ fst e }> ~>  <{ fst e' }>
-
-| step_snd : forall e e',
-  e ~> e' ->
-  <{ snd e }> ~>  <{ snd e' }>
-
-| step_pairL : forall e1 e1' e2,
-  e1 ~> e1' ->
-  <{ ⟨ e1, e2 ⟩ }> ~>  <{ ⟨ e1', e2 ⟩  }>
-
-| step_pairR : forall v e e',
-  is_val v ->
-  e ~> e' ->
-  <{ ⟨ v, e ⟩ }> ~>  <{ ⟨ v, e' ⟩  }>
-
+  <{ if e then e1 else e2 }> ~> <{ if e' then e1 else e2 }>
 | step_lam_head : forall f f' e,
   f ~> f' ->
   <{ f e }> ~>  <{ f' e }>
@@ -42,9 +23,6 @@ Inductive step : expr -> expr -> Prop :=
   is_val f ->
   e ~> e' ->
   <{ f e }> ~>  <{ f e' }>
-| step_tlam_head : forall e e',
-  e ~> e' ->
-  <{ e _ }> ~>  <{ e' _ }>
 where "t '~>' t'" := (step t t').
 Hint Constructors step : core.
 
@@ -55,32 +33,6 @@ Notation "t '~>*' t'" := (mstep t t') (at level 60).
 (*   ∃ e', step e e'. *)
 
 (** Examples *)
-Goal <{ (λ x , x) tt }> ~>* <{tt}>.
-Proof.
-  eapply star_one.
-  apply step_lam_red.
-  apply v_unit.
-Qed.
-
-Goal <{ fst ((λ x , ( ⟨ (λ y , tt) x , (λ y , x) tt⟩ )) tt)}> ~>* <{tt}>.
-Proof.
-  eapply star_trans with <{ fst ( ⟨ (λ y , tt) tt , (λ y , tt) tt⟩ )}>.
-  eapply star_one.
-  eapply step_fst; eapply step_lam_red ; apply v_unit.
-
-  eapply star_trans with <{ fst ( ⟨ tt , (λ y , tt) tt⟩ )}>.
-  eapply star_one.
-  eapply step_fst; eapply step_pairL; eapply (step_lam_red y <{ tt }> ); apply v_unit.
-
-  eapply star_trans with <{ fst ( ⟨ tt , tt⟩ )}>.
-  eapply star_one.
-  eapply step_fst; eapply step_pairR;[apply v_unit|];
-    eapply (step_lam_red y <{ tt }> ); apply v_unit.
-
-  eapply star_one.
-  eapply step_fst_red; apply v_unit.
-Qed.
-
 Lemma identity : forall v e, e = (of_val v) -> <{ (λ x , x) e }> ~>* <{e}>.
 Proof.
   intros v e ->.
@@ -94,8 +46,6 @@ Proof.
   intros e e' val_e.
   generalize dependent e'.
   induction e; intros e' step; try inversion val_e;inversion step; subst.
-  - eapply IHe1 in H1; eapply H1; eauto.
-  - eapply IHe2 in H2; eapply H2; eauto.
 Qed.
 
 Lemma is_val_step : forall e e', is_val e -> e ~>* e' -> e' = e.
@@ -105,12 +55,12 @@ Lemma is_val_step : forall e e', is_val e -> e ~>* e' -> e' = e.
 Qed.
 
 Ltac solve_by_inverts n :=
-  match goal with | H : ?T |- _ =>
-                      match type of T with Prop =>
-                                             solve [
-                                                 inversion H;
-                                                 match n with S (S (?n')) => subst; solve_by_inverts (S n') end ]
-                      end end.
+  match goal with
+  | H : ?T |- _ =>
+      match type of T with Prop =>
+      solve [inversion H; match n with S (S (?n')) => subst; solve_by_inverts (S n') end ]
+      end
+  end.
 
 Lemma sf_deterministic : deterministic expr step.
 Proof.
@@ -118,26 +68,16 @@ Proof.
   generalize dependent e''.
   induction step_e'; intros e'' step_e''.
   - inversion step_e''; subst; auto.
-    + inversion H2; subst; apply is_val_stuck in H2; auto; contradiction.
+    + inversion H3; subst; apply is_val_stuck in H3; auto; contradiction.
   - inversion step_e''; subst; auto.
-    inversion H2; subst; apply is_val_stuck in H2; auto; contradiction.
+    inversion H3; subst; apply is_val_stuck in H3; auto; contradiction.
   - inversion step_e''; subst; auto.
     + inversion H3.
     + apply is_val_stuck in H4; auto; contradiction.
   - inversion step_e''; subst; auto.
-    apply is_val_stuck in H0; auto; contradiction.
-  - inversion step_e'';subst.
-    apply is_val_stuck in step_e'; auto; contradiction.
-    eapply IHstep_e' in H0; subst;auto.
-  - inversion step_e'';subst.
-    apply is_val_stuck in step_e'; auto; contradiction.
-    eapply IHstep_e' in H0; subst;auto.
-  - inversion step_e'';subst.
-    eapply IHstep_e' in H2; subst;auto.
-    apply is_val_stuck in step_e'; auto; contradiction.
-  - inversion step_e'';subst.
-    apply is_val_stuck in H3; auto; contradiction.
-    eapply IHstep_e' in H4; subst;auto.
+    + apply is_val_stuck in step_e'; auto; contradiction.
+    + apply is_val_stuck in step_e'; auto; contradiction.
+    + eapply IHstep_e' in H3; subst;auto.
   - inversion step_e'';subst.
     apply is_val_stuck in step_e'; auto; contradiction.
     eapply IHstep_e' in H2; subst;auto.
@@ -146,9 +86,6 @@ Proof.
     apply is_val_stuck in step_e'; auto; contradiction.
     apply is_val_stuck in H3; auto; contradiction.
     eapply IHstep_e' in H4; subst;auto.
-  - inversion step_e'';subst.
-    apply is_val_stuck in step_e'; auto; contradiction.
-    eapply IHstep_e' in H0; subst;auto.
 Qed.
 
 Lemma star_step : forall e e2 e3,
