theories/syntax_stlc.v
@@ -1,0 +1,173 @@
+Set Warnings "-notation-overridden,-parsing,-deprecated-hint-without-locality".
+From Coq Require Import Strings.String.
+From stdpp Require Import gmap list.
+From logical_relation Require Import relation.
+
+Inductive ty : Type :=
+| Ty_Bool : ty
+| Ty_Arrow : ty -> ty -> ty.
+
+Inductive expr : Type :=
+| expr_var : string -> expr
+| expr_true : expr
+| expr_false : expr
+| expr_if : expr -> expr -> expr -> expr
+| expr_app : expr -> expr -> expr
+| expr_abs : string -> expr -> expr.
+Inductive val :=
+| val_true : val
+| val_false : val
+| val_abs : string -> expr -> val.
+
+Fixpoint of_val (v : val) : expr :=
+  match v with
+  | val_true => expr_true
+  | val_false => expr_false
+  | val_abs s e => expr_abs s e
+  end.
+
+Fixpoint to_val (e : expr) : option val :=
+  match e with
+  | expr_true => Some val_true
+  | expr_false => Some val_false
+  | expr_abs s e => Some (val_abs s e)
+  | _ => None
+  end.
+
+Inductive is_val : expr -> Prop :=
+| v_true : is_val expr_true
+| v_false : is_val expr_false
+| v_abs : forall x t1, is_val (expr_abs x t1).
+
+Hint Constructors is_val : core.
+
+
+(** Equality  *)
+Lemma to_of_val v : to_val (of_val v) = Some v.
+Proof.
+  by induction v; simplify_option_eq; repeat f_equal; try apply (proof_irrel _).
+Qed.
+
+Lemma of_to_val e v : to_val e = Some v → of_val v = e.
+Proof.
+  revert v; induction e; intros v ?; simplify_option_eq; auto with f_equal.
+Qed.
+
+Lemma is_val_of_val: forall v, is_val (of_val v).
+Proof.
+  intros.
+  induction v; simpl; auto.
+Qed.
+
+
+Declare Custom Entry stlc.
+Notation "<{ e }>" := e (e custom stlc at level 99).
+Notation "x" := x (in custom stlc at level 0, x constr at level 0).
+Notation "S -> T" := (Ty_Arrow S T) (in custom stlc at level 50, right associativity).
+Notation "'Bool'" := Ty_Bool (in custom stlc at level 50, right associativity).
+Coercion expr_var : string >-> expr.
+Notation "'true'" := expr_true (in custom stlc at level 0).
+Notation "'false'" := expr_false (in custom stlc at level 0).
+Notation "e1 e2" := (expr_app e1 e2) (in custom stlc at level 1, left associativity).
+Notation "'λ' x ',' y" :=
+  (expr_abs x y) (in custom stlc at level 90, x at level 99,
+        y custom stlc at level 99,
+        left associativity).
+Notation "'if' x 'then' y 'else' z" :=
+  (expr_if x y z) (in custom stlc at level 89,
+                    x custom stlc at level 99,
+                    y custom stlc at level 99,
+                    z custom stlc at level 99,
+                    left associativity).
+Definition x : string := "x".
+Definition y : string := "y".
+Definition z : string := "z".
+Hint Unfold x : core.
+Hint Unfold y : core.
+Hint Unfold z : core.
+
+Fixpoint subst_term (x : string) (s : expr) (t : expr) : expr :=
+  match t with
+  | expr_var y =>
+      if String.eqb x y then s else t
+  | <{ true }> =>  <{ true }>
+  | <{ false }> =>  <{ false }>
+  | <{ if e then e1 else e2 }> =>
+      <{ if (subst_term x s e) then (subst_term x s e1) else (subst_term x s e2) }>
+  | <{ t1 t2 }> =>
+      <{ (subst_term x s t1) (subst_term x s t2) }>
+  | <{ λ y, t1 }> =>
+      if String.eqb x y then t else <{ λ y, (subst_term x s t1) }>
+  end.
+
+Notation "'[' x '/' s ']' t" := (subst_term x s t) (in custom stlc at level 20).
+
+Definition context := gmap string ty.
+
+(* TODO notation / definition for the empty context and tcontext *)
+
+Reserved Notation " Γ '⊢' t '∈' T"
+  (at level 101, t custom stlc, T custom stlc at level 0).
+
+Inductive appears_free_in (x : string) : expr → Prop :=
+| afi_var : appears_free_in x <{x}>
+| afi_if_cond : ∀ e e1 e2,
+  appears_free_in x e →
+  appears_free_in x <{ if e then e1 else e2 }>
+| afi_if1 : ∀ e e1 e2,
+  appears_free_in x e1 →
+  appears_free_in x <{ if e then e1 else e2 }>
+| afi_if2 : ∀ e e1 e2,
+  appears_free_in x e2 →
+  appears_free_in x <{ if e then e1 else e2 }>
+| afi_app1 : ∀ t1 t2,
+  appears_free_in x t1 →
+  appears_free_in x <{t1 t2}>
+| afi_app2 : ∀ t1 t2,
+  appears_free_in x t2 →
+  appears_free_in x <{t1 t2}>
+| afi_abs : ∀ y t1,
+  y ≠ x →
+  appears_free_in x t1 →
+  appears_free_in x <{ λ y, t1}>.
+
+Inductive typing_judgment : context -> expr -> ty -> Prop :=
+| T_True: forall Γ, Γ ⊢ true ∈ Bool
+| T_False: forall Γ, Γ ⊢ false ∈ Bool
+| T_Var: forall Γ τ (x : string), Γ !! x = Some τ -> Γ ⊢ x ∈ τ
+| T_Lam: forall Γ x e τ1 τ2,
+  x ∉ dom Γ ->
+  (<[x:=τ1]> Γ) ⊢ e ∈ τ2 ->
+    Γ ⊢ <{ λ x , e }> ∈ <{ τ1 -> τ2 }>
+| T_App: forall Γ e e' τ1 τ2,
+  Γ ⊢ e ∈ <{ τ1 -> τ2 }> ->
+    Γ ⊢ e' ∈ τ1 ->
+      Γ ⊢ e e' ∈ τ2
+| T_If: forall Γ e e1 e2 τ,
+    Γ ⊢ e ∈ <{ Bool }> ->
+    Γ ⊢ e1 ∈ τ ->
+    Γ ⊢ e2 ∈ τ ->
+      Γ ⊢ <{ if e then e1 else e2 }> ∈ τ
+where "Γ '⊢' t '∈' T" := (typing_judgment Γ t T).
+Hint Constructors typing_judgment : core.
+
+Notation "( x )" := x (in custom stlc, x at level 99).
+
+Lemma canonical_forms_bool : ∀ e,
+  ∅ ⊢ e ∈ Bool →
+  is_val e →
+  (e = <{true}>) ∨ (e = <{false}>).
+Proof.
+  intros.
+  destruct H0;auto. inversion H.
+Qed.
+
+ Lemma canonical_forms_fun : ∀ t T1 T2,
+  ∅ ⊢ t ∈ <{  (T1 -> T2) }> →
+  is_val t →
+  ∃ x u, t = <{ λ x, u }>.
+Proof.
+  intros t T1 T2 HT HVal.
+  destruct HVal as [x ? t1| |] ; inversion HT; subst.
+  exists x0, t1. reflexivity.
+Qed.
